src/impl/TLS13.Impl.Server.Network.fsti
@@ -17,6 +17,7 @@ module ST = TLS13.Impl.Server.Types
 module Seq = FStar.Seq
 module SZ = FStar.SizeT
 module U8 = FStar.UInt8
+module W = TLS13.Wire.Spec
 
 type server = CR.connection_state
 
@@ -189,4 +190,6 @@ fn process_network_bytes
                    buffer_resp
                    (Ghost.reveal 'raw_bytes)
                    network_out_bytes
-                   app_out_bytes)
+                   app_out_bytes /\
+                (buffer_resp.ST.response.ST.status == ST.NeedMoreInput ==>
+                  W.parse_record_wire (Ghost.reveal 'raw_bytes) == None))
