src/impl/TLS13.Impl.Server.fst
@@ -3284,7 +3284,9 @@ fn process_network_bytes
                    buffer_resp
                    (Ghost.reveal 'raw_bytes)
                    network_out_bytes
-                   app_out_bytes)
+                   app_out_bytes /\
+                (buffer_resp.ST.response.ST.status == ST.NeedMoreInput ==>
+                  W.parse_record_wire (Ghost.reveal 'raw_bytes) == None))
 {
   rewrite (connection_exactly s 'st0) as (SN.connection_exactly s 'st0);
   let buffer_resp = SN.process_network_bytes
@@ -3300,6 +3302,8 @@ fn process_network_bytes
             pts_to raw 'raw_bytes **
             pts_to network_out network_out_bytes **
             pts_to app_out app_out_bytes);
+  assert (pure (buffer_resp.ST.response.ST.status == ST.NeedMoreInput ==>
+    W.parse_record_wire (Ghost.reveal 'raw_bytes) == None));
   rewrite (SN.connection_exactly s st1) as (connection_exactly s st1);
   buffer_resp
 }
